---


---

<h2 id="distance"><strong>Distance</strong></h2>
<p><strong>Exercice 1</strong><br>
Prouvons que les trois axiomes <span class="katex--inline"><span class="katex"><span class="katex-mathml"><math><semantics><mrow><mi>A</mi><mn>1</mn></mrow><annotation encoding="application/x-tex">A1</annotation></semantics></math></span><span class="katex-html" aria-hidden="true"><span class="base"><span class="strut" style="height: 0.68333em; vertical-align: 0em;"></span><span class="mord mathdefault">A</span><span class="mord">1</span></span></span></span></span> à <span class="katex--inline"><span class="katex"><span class="katex-mathml"><math><semantics><mrow><mi>A</mi><mn>3</mn></mrow><annotation encoding="application/x-tex">A3</annotation></semantics></math></span><span class="katex-html" aria-hidden="true"><span class="base"><span class="strut" style="height: 0.68333em; vertical-align: 0em;"></span><span class="mord mathdefault">A</span><span class="mord">3</span></span></span></span></span> impliquent la condition de non-négativité :<br>
<span class="katex--display"><span class="katex-display"><span class="katex"><span class="katex-mathml"><math><semantics><mrow><mi>d</mi><mo stretchy="false">(</mo><mi>x</mi><mo separator="true">,</mo><mi>y</mi><mo stretchy="false">)</mo><mo>≥</mo><mn>0.</mn></mrow><annotation encoding="application/x-tex">d(x,y) \geq 0.</annotation></semantics></math></span><span class="katex-html" aria-hidden="true"><span class="base"><span class="strut" style="height: 1em; vertical-align: -0.25em;"></span><span class="mord mathdefault">d</span><span class="mopen">(</span><span class="mord mathdefault">x</span><span class="mpunct">,</span><span class="mspace" style="margin-right: 0.166667em;"></span><span class="mord mathdefault" style="margin-right: 0.03588em;">y</span><span class="mclose">)</span><span class="mspace" style="margin-right: 0.277778em;"></span><span class="mrel">≥</span><span class="mspace" style="margin-right: 0.277778em;"></span></span><span class="base"><span class="strut" style="height: 0.64444em; vertical-align: 0em;"></span><span class="mord">0</span><span class="mord">.</span></span></span></span></span></span></p>
<p><em>Preuve</em><br>
On a d’après <span class="katex--inline"><span class="katex"><span class="katex-mathml"><math><semantics><mrow><mi>A</mi><mn>3</mn></mrow><annotation encoding="application/x-tex">A3</annotation></semantics></math></span><span class="katex-html" aria-hidden="true"><span class="base"><span class="strut" style="height: 0.68333em; vertical-align: 0em;"></span><span class="mord mathdefault">A</span><span class="mord">3</span></span></span></span></span> : <span class="katex--display"><span class="katex-display"><span class="katex"><span class="katex-mathml"><math><semantics><mrow><mi>d</mi><mo stretchy="false">(</mo><mi>x</mi><mo separator="true">,</mo><mi>z</mi><mo stretchy="false">)</mo><mo>≤</mo><mi>d</mi><mo stretchy="false">(</mo><mi>x</mi><mo separator="true">,</mo><mi>y</mi><mo stretchy="false">)</mo><mo>+</mo><mi>d</mi><mo stretchy="false">(</mo><mi>y</mi><mo separator="true">,</mo><mi>z</mi><mo stretchy="false">)</mo></mrow><annotation encoding="application/x-tex">d(x,z)\leq d(x,y)+d(y,z) </annotation></semantics></math></span><span class="katex-html" aria-hidden="true"><span class="base"><span class="strut" style="height: 1em; vertical-align: -0.25em;"></span><span class="mord mathdefault">d</span><span class="mopen">(</span><span class="mord mathdefault">x</span><span class="mpunct">,</span><span class="mspace" style="margin-right: 0.166667em;"></span><span class="mord mathdefault" style="margin-right: 0.04398em;">z</span><span class="mclose">)</span><span class="mspace" style="margin-right: 0.277778em;"></span><span class="mrel">≤</span><span class="mspace" style="margin-right: 0.277778em;"></span></span><span class="base"><span class="strut" style="height: 1em; vertical-align: -0.25em;"></span><span class="mord mathdefault">d</span><span class="mopen">(</span><span class="mord mathdefault">x</span><span class="mpunct">,</span><span class="mspace" style="margin-right: 0.166667em;"></span><span class="mord mathdefault" style="margin-right: 0.03588em;">y</span><span class="mclose">)</span><span class="mspace" style="margin-right: 0.222222em;"></span><span class="mbin">+</span><span class="mspace" style="margin-right: 0.222222em;"></span></span><span class="base"><span class="strut" style="height: 1em; vertical-align: -0.25em;"></span><span class="mord mathdefault">d</span><span class="mopen">(</span><span class="mord mathdefault" style="margin-right: 0.03588em;">y</span><span class="mpunct">,</span><span class="mspace" style="margin-right: 0.166667em;"></span><span class="mord mathdefault" style="margin-right: 0.04398em;">z</span><span class="mclose">)</span></span></span></span></span></span><br>
ce qui implique que :    <span class="katex--display"><span class="katex-display"><span class="katex"><span class="katex-mathml"><math><semantics><mrow><mi>d</mi><mo stretchy="false">(</mo><mi>x</mi><mo separator="true">,</mo><mi>y</mi><mo stretchy="false">)</mo><mo>≥</mo><mi>d</mi><mo stretchy="false">(</mo><mi>x</mi><mo separator="true">,</mo><mi>z</mi><mo stretchy="false">)</mo><mo>−</mo><mi>d</mi><mo stretchy="false">(</mo><mi>y</mi><mo separator="true">,</mo><mi>z</mi><mo stretchy="false">)</mo></mrow><annotation encoding="application/x-tex">d(x,y) \geq d(x,z) - d(y,z)</annotation></semantics></math></span><span class="katex-html" aria-hidden="true"><span class="base"><span class="strut" style="height: 1em; vertical-align: -0.25em;"></span><span class="mord mathdefault">d</span><span class="mopen">(</span><span class="mord mathdefault">x</span><span class="mpunct">,</span><span class="mspace" style="margin-right: 0.166667em;"></span><span class="mord mathdefault" style="margin-right: 0.03588em;">y</span><span class="mclose">)</span><span class="mspace" style="margin-right: 0.277778em;"></span><span class="mrel">≥</span><span class="mspace" style="margin-right: 0.277778em;"></span></span><span class="base"><span class="strut" style="height: 1em; vertical-align: -0.25em;"></span><span class="mord mathdefault">d</span><span class="mopen">(</span><span class="mord mathdefault">x</span><span class="mpunct">,</span><span class="mspace" style="margin-right: 0.166667em;"></span><span class="mord mathdefault" style="margin-right: 0.04398em;">z</span><span class="mclose">)</span><span class="mspace" style="margin-right: 0.222222em;"></span><span class="mbin">−</span><span class="mspace" style="margin-right: 0.222222em;"></span></span><span class="base"><span class="strut" style="height: 1em; vertical-align: -0.25em;"></span><span class="mord mathdefault">d</span><span class="mopen">(</span><span class="mord mathdefault" style="margin-right: 0.03588em;">y</span><span class="mpunct">,</span><span class="mspace" style="margin-right: 0.166667em;"></span><span class="mord mathdefault" style="margin-right: 0.04398em;">z</span><span class="mclose">)</span></span></span></span></span></span><br>
et d’après <span class="katex--inline"><span class="katex"><span class="katex-mathml"><math><semantics><mrow><mi>A</mi><mn>2</mn></mrow><annotation encoding="application/x-tex">A2</annotation></semantics></math></span><span class="katex-html" aria-hidden="true"><span class="base"><span class="strut" style="height: 0.68333em; vertical-align: 0em;"></span><span class="mord mathdefault">A</span><span class="mord">2</span></span></span></span></span> , <span class="katex--display"><span class="katex-display"><span class="katex"><span class="katex-mathml"><math><semantics><mrow><mi>d</mi><mo stretchy="false">(</mo><mi>x</mi><mo separator="true">,</mo><mi>y</mi><mo stretchy="false">)</mo><mo>≥</mo><mi>d</mi><mo stretchy="false">(</mo><mi>z</mi><mo separator="true">,</mo><mi>x</mi><mo stretchy="false">)</mo><mo>−</mo><mi>d</mi><mo stretchy="false">(</mo><mi>z</mi><mo separator="true">,</mo><mi>y</mi><mo stretchy="false">)</mo></mrow><annotation encoding="application/x-tex">d(x,y) \geq d(z,x) - d(z,y)</annotation></semantics></math></span><span class="katex-html" aria-hidden="true"><span class="base"><span class="strut" style="height: 1em; vertical-align: -0.25em;"></span><span class="mord mathdefault">d</span><span class="mopen">(</span><span class="mord mathdefault">x</span><span class="mpunct">,</span><span class="mspace" style="margin-right: 0.166667em;"></span><span class="mord mathdefault" style="margin-right: 0.03588em;">y</span><span class="mclose">)</span><span class="mspace" style="margin-right: 0.277778em;"></span><span class="mrel">≥</span><span class="mspace" style="margin-right: 0.277778em;"></span></span><span class="base"><span class="strut" style="height: 1em; vertical-align: -0.25em;"></span><span class="mord mathdefault">d</span><span class="mopen">(</span><span class="mord mathdefault" style="margin-right: 0.04398em;">z</span><span class="mpunct">,</span><span class="mspace" style="margin-right: 0.166667em;"></span><span class="mord mathdefault">x</span><span class="mclose">)</span><span class="mspace" style="margin-right: 0.222222em;"></span><span class="mbin">−</span><span class="mspace" style="margin-right: 0.222222em;"></span></span><span class="base"><span class="strut" style="height: 1em; vertical-align: -0.25em;"></span><span class="mord mathdefault">d</span><span class="mopen">(</span><span class="mord mathdefault" style="margin-right: 0.04398em;">z</span><span class="mpunct">,</span><span class="mspace" style="margin-right: 0.166667em;"></span><span class="mord mathdefault" style="margin-right: 0.03588em;">y</span><span class="mclose">)</span></span></span></span></span></span><br>
donc<br>
<span class="katex--display"><span class="katex-display"><span class="katex"><span class="katex-mathml"><math><semantics><mrow><mi>d</mi><mo stretchy="false">(</mo><mi>x</mi><mo separator="true">,</mo><mi>y</mi><mo stretchy="false">)</mo><mo>≥</mo><mi>d</mi><mo stretchy="false">(</mo><mi>z</mi><mo separator="true">,</mo><mi>x</mi><mo stretchy="false">)</mo><mo>−</mo><mi>d</mi><mo stretchy="false">(</mo><mi>z</mi><mo separator="true">,</mo><mi>y</mi><mo stretchy="false">)</mo><mo>≥</mo><mo>−</mo><mi>d</mi><mo stretchy="false">(</mo><mi>z</mi><mo separator="true">,</mo><mi>z</mi><mo stretchy="false">)</mo><mo>=</mo><mn>0</mn></mrow><annotation encoding="application/x-tex">d(x,y) \geq d(z,x) - d(z,y) \geq -d(z,z)=0</annotation></semantics></math></span><span class="katex-html" aria-hidden="true"><span class="base"><span class="strut" style="height: 1em; vertical-align: -0.25em;"></span><span class="mord mathdefault">d</span><span class="mopen">(</span><span class="mord mathdefault">x</span><span class="mpunct">,</span><span class="mspace" style="margin-right: 0.166667em;"></span><span class="mord mathdefault" style="margin-right: 0.03588em;">y</span><span class="mclose">)</span><span class="mspace" style="margin-right: 0.277778em;"></span><span class="mrel">≥</span><span class="mspace" style="margin-right: 0.277778em;"></span></span><span class="base"><span class="strut" style="height: 1em; vertical-align: -0.25em;"></span><span class="mord mathdefault">d</span><span class="mopen">(</span><span class="mord mathdefault" style="margin-right: 0.04398em;">z</span><span class="mpunct">,</span><span class="mspace" style="margin-right: 0.166667em;"></span><span class="mord mathdefault">x</span><span class="mclose">)</span><span class="mspace" style="margin-right: 0.222222em;"></span><span class="mbin">−</span><span class="mspace" style="margin-right: 0.222222em;"></span></span><span class="base"><span class="strut" style="height: 1em; vertical-align: -0.25em;"></span><span class="mord mathdefault">d</span><span class="mopen">(</span><span class="mord mathdefault" style="margin-right: 0.04398em;">z</span><span class="mpunct">,</span><span class="mspace" style="margin-right: 0.166667em;"></span><span class="mord mathdefault" style="margin-right: 0.03588em;">y</span><span class="mclose">)</span><span class="mspace" style="margin-right: 0.277778em;"></span><span class="mrel">≥</span><span class="mspace" style="margin-right: 0.277778em;"></span></span><span class="base"><span class="strut" style="height: 1em; vertical-align: -0.25em;"></span><span class="mord">−</span><span class="mord mathdefault">d</span><span class="mopen">(</span><span class="mord mathdefault" style="margin-right: 0.04398em;">z</span><span class="mpunct">,</span><span class="mspace" style="margin-right: 0.166667em;"></span><span class="mord mathdefault" style="margin-right: 0.04398em;">z</span><span class="mclose">)</span><span class="mspace" style="margin-right: 0.277778em;"></span><span class="mrel">=</span><span class="mspace" style="margin-right: 0.277778em;"></span></span><span class="base"><span class="strut" style="height: 0.64444em; vertical-align: 0em;"></span><span class="mord">0</span></span></span></span></span></span><br>
d’où<br>
<span class="katex--display"><span class="katex-display"><span class="katex"><span class="katex-mathml"><math><semantics><mrow><mi>d</mi><mo stretchy="false">(</mo><mi>x</mi><mo separator="true">,</mo><mi>y</mi><mo stretchy="false">)</mo><mo>≥</mo><mn>0.</mn></mrow><annotation encoding="application/x-tex">d(x,y) \geq 0.</annotation></semantics></math></span><span class="katex-html" aria-hidden="true"><span class="base"><span class="strut" style="height: 1em; vertical-align: -0.25em;"></span><span class="mord mathdefault">d</span><span class="mopen">(</span><span class="mord mathdefault">x</span><span class="mpunct">,</span><span class="mspace" style="margin-right: 0.166667em;"></span><span class="mord mathdefault" style="margin-right: 0.03588em;">y</span><span class="mclose">)</span><span class="mspace" style="margin-right: 0.277778em;"></span><span class="mrel">≥</span><span class="mspace" style="margin-right: 0.277778em;"></span></span><span class="base"><span class="strut" style="height: 0.64444em; vertical-align: 0em;"></span><span class="mord">0</span><span class="mord">.</span></span></span></span></span></span></p>

